RelationalAlgebra/Equivalence/RAtoFOL/Projection.lean
@@ -16,19 +16,32 @@ theorem ra_to_fol_evalT.p_def.mp (h : RA.Query.isWellTyped dbi.schema (.p rs q))
       have h_rs : ↑rs ⊆ t.Dom := by
         rw [Set.subset_def]
         intro x hx
-        simp_all only [FOL.Query.RealizeDom.def, ra_to_fol_query.isWellTyped, ra_to_fol_query_schema, and_imp,
-          forall_const, true_and, dite_not, Finset.mem_coe, PFun.mem_dom, Part.dom_iff_mem]
+        simp_all only [FOL.Query.RealizeDom.def, ra_to_fol_query.isWellTyped,
+          ra_to_fol_query_schema, and_imp, forall_const, true_and, dite_not, Part.dom_iff_mem,
+          Finset.mem_coe, PFun.mem_dom]
         exact h_t_dom x x (right hx) (by simp [hx])
       use t.restrict h_rs
       simp_all only [FOL.Query.RealizeDom.def, ra_to_fol_query.isWellTyped, ra_to_fol_query_schema,
         and_imp, forall_const, projectAttribute, Finset.mem_sdiff, true_and, dite_not]
       apply And.intro
       · apply ih
-        . simp_all only [ra_to_fol_query.isWellTyped, FOL.BoundedQuery.Realize.exs_def,
-          FOL.BoundedQuery.Realize.relabel_def, Nat.add_zero, Fin.castAdd_zero, Fin.cast_refl,
-          CompTriple.comp_eq]
-          obtain ⟨w, h⟩ := a_2
-          sorry
+        . have ⟨dropSet, h_dropSet⟩ : ∃s, (FOL.BoundedQuery.schema (ra_to_fol_query q dbi.schema) \ rs) = s := by simp
+          induction dropSet using Finset.induction_on with
+          | empty =>
+            rw [h_dropSet] at a_2
+            unfold projectAttribute at a_2
+            simp at a_2
+            have z : rs = q.schema dbi.schema := by simp_all; exact Finset.Subset.antisymm right h_dropSet
+            have h_rs' : ↑(FOL.BoundedQuery.schema (ra_to_fol_query q dbi.schema)) ⊆ PFun.Dom t := by simp_all
+            have z' := FOL.BoundedQuery.Realize.tuple_restrict2
+              (ra_to_fol_query.isWellTyped q dbi.schema left)
+              (h_rs')
+              a_2
+            have : (PFun.restrict t h_rs) = (PFun.restrict t h_rs') := by aesop
+            simp [this, z']
+          | insert h ih =>
+            rename_i a ds
+            sorry
         . exact right
       · intro a
         apply And.intro
@@ -59,19 +72,22 @@ theorem ra_to_fol_evalT.p_def.mpr (h : RA.Query.isWellTyped dbi.schema (.p rs q)
           (by simp_all)
 
       simp only [ra_to_fol_query]
-      simp_all only [RA.Query.isWellTyped.p_def, RA.Query.evaluateT.p_def, projectionT,
-        Set.mem_setOf_eq, forall_const]
-      simp_all only [projectQuery.def, Nat.add_zero]
-      simp_all only [FOL.Query.RealizeDom.def, ra_to_fol_query.isWellTyped, ra_to_fol_query_schema]
-      obtain ⟨left, right⟩ := h
-      obtain ⟨w, h⟩ := h_RA_eval
-      obtain ⟨hw, right_1⟩ := h
+      have : t = t.restrict (Set.Subset.antisymm_iff.mp t_Dom.symm).1 := by simp_all
+      rw [this]
+      apply projectQuery.Realize_restrict_def
+      . simp at h
+        obtain ⟨left, right⟩ := h
+        exact ra_to_fol_query.isWellTyped q dbi.schema left
+      . simp_all [projectionT]
+        obtain ⟨left, right⟩ := h
+        obtain ⟨w, h⟩ := h_RA_eval
+        obtain ⟨left_1, right_1⟩ := h
 
-      have z := (ih w hw)
-      have w_Dom : w.Dom = q.schema dbi.schema := by
-        exact RA.Query.evaluate.validSchema q left w hw
-
-      simp_all only [ra_to_fol_query.isWellTyped, subset_refl, and_self,
-        FOL.BoundedQuery.Realize.exs_def, FOL.BoundedQuery.Realize.relabel_def, Nat.add_zero,
-        Fin.castAdd_zero, Fin.cast_refl, CompTriple.comp_eq]
-      sorry
+        have : t = w := by
+          ext a v
+          by_cases a ∈ rs
+          . aesop
+          . sorry
+            -- ???
+        rw [this]
+        exact (ih w left_1).1
